update npbc_check to split types of steps

examples/pseudo_bool/npbc_checkScript.sml
@@ -39,41 +39,23 @@ Datatype:
   | Weak constr var     (* Addition of literal axioms until "var" disappears *)
 End
 
-Type subst = ``:(bool + num lit) num_map``;
-
+(* Steps that preserve logical implication *)
 Datatype:
-  pbpstep =
+  lstep =
   | Contradiction num (* Id representing a contradiction *)
   | Delete (num list) (* Ids to to delete *)
   | Cutting constr    (* Adds a constraint using cutting planes, written in reverse polish notation *)
-  | Con npbc (pbpstep list) (* Prove constraint by contradiction *)
-  | Red npbc subst (( (num + unit) option,pbpstep list) alist) (* Redundancy step: for simplicity, the first subgoal is stored as SOME 0 *)
+  | Con npbc (lstep list) (* Prove constraint by contradiction *)
   | Check num npbc    (* Debugging / other steps are parsed as no ops *)
-  | NoOp              (* Debugging / other steps are parsed as no ops *)
+  | NoOp              (* Other steps are parsed as no ops *)
 End
 
-Definition pbpstep_ok_def[simp]:
-  (pbpstep_ok (Con n pfs) ⇔
-    compact n ∧ (EVERY pbpstep_ok pfs)) ∧
-  (pbpstep_ok (Red n _ pfs) ⇔
-    compact n ∧ EVERY (EVERY pbpstep_ok) (MAP SND pfs)) ∧
-  (pbpstep_ok _ ⇔ T)
+Definition lstep_ok_def[simp]:
+  (lstep_ok (Con n pfs) ⇔
+    compact n ∧ (EVERY lstep_ok pfs)) ∧
+  (lstep_ok _ ⇔ T)
 Termination
-  WF_REL_TAC ‘measure pbpstep_size’ \\ rw []
-  \\ gvs [fetch "-" "pbpstep_size_eq"] \\ rw []
-  \\ imp_res_tac MEM_list_size
-  \\ pop_assum (qspec_then`list_size pbpstep_size` mp_tac)
-  \\ pop_assum (qspec_then`pbpstep_size` assume_tac)
-  \\ rw[]
-  \\ qmatch_goalsub_abbrev_tac`_ < _ + (_ + (ls2 + _))`
-  \\ qmatch_asmsub_abbrev_tac`_ < ls1`
-  \\ `ls1 <= ls2` by (
-    unabbrev_all_tac
-    \\ rpt (pop_assum kall_tac)
-    \\ Induct_on`pfs` \\ simp[FORALL_PROD]
-    \\ rw[] \\ EVAL_TAC
-    \\ fs[])
-  \\ fs[]
+  WF_REL_TAC ‘measure lstep_size’ \\ rw []
 End
 
 (*
@@ -81,7 +63,6 @@ End
   num -> pbc
 *)
 Type pbf = ``:npbc spt``;
-Type pbp = ``:pbpstep list``;
 
 Definition check_cutting_def:
   (check_cutting fml (Id n) = lookup n fml) ∧
@@ -101,80 +82,25 @@ Definition check_cutting_def:
     OPTION_MAP (λc. weaken c var) (check_cutting fml c))
 End
 
-(* A simple datatype for checking pbp
-  The result is either:
-  Unsat num    : unsatisfiability proved, continue with next ID
-  Fail         : proof step failed (more errors can be added in imperative part)
-  Cont 'a num : continue with state 'a and next ID (input formula is sat equiv to the pbv)
+(* The result of a checking step is either:
+  Fail        : proof step failed
+  Unsat num   : unsatisfiability proved, continue with next ID
+  Cont 'a num : continue with state 'a and next ID
 *)
 Datatype:
   pbpres = Unsat num | Fail | Cont 'a num
 End
 
-Definition subst_fun_def:
-  subst_fun (s:subst) n = lookup n s
-End
-
-Definition is_pol_con_def[simp]:
-  is_pol_con (Cutting _) = T ∧
-  is_pol_con (Contradiction _) = T ∧
-  is_pol_con (Con _ _) = T ∧
-  is_pol_con (Check _ _) = T ∧
-  is_pol_con _ = F
-End
-
-Definition map_opt_def:
-  map_opt f LN = LN ∧
-  map_opt f (LS x) = (case f x of NONE => LN | SOME a => LS a) ∧
-  map_opt f (BN t1 t2) = mk_BN (map_opt f t1) (map_opt f t2) ∧
-  map_opt f (BS t1 x t2) =
-    case f x of
-    | NONE => mk_BN (map_opt f t1) (map_opt f t2)
-    | SOME a => mk_BS (map_opt f t1) a (map_opt f t2)
-End
-
-Definition fold_opt_def:
-  (fold_opt f i [] = SOME i) ∧
-  (fold_opt f i (x::xs) =
-    case f i x of NONE => NONE
-    | SOME id' => fold_opt f id' xs)
-End
-
-(* Apply a substitution where needed *)
-Definition extract_clauses_def:
-  (extract_clauses f def fml [] acc = SOME (REVERSE acc)) ∧
-  (extract_clauses f def fml (cpf::pfs) acc =
-    case cpf of
-      (NONE,pf) => extract_clauses f def fml pfs ((NONE,pf)::acc)
-    | (SOME (INL n),pf) =>
-      (case lookup n fml of
-        NONE => NONE
-      | SOME c => extract_clauses f def fml pfs ((SOME (subst f c),pf)::acc))
-    | (SOME (INR u),pf) =>
-      extract_clauses f def fml pfs ((SOME (subst f def),pf)::acc))
-End
-
-Theorem extract_clauses_MAP_SND:
-  ∀f def fml pfs acc res.
-  extract_clauses f def fml pfs acc = SOME res ⇒
-  MAP SND res =  REVERSE (MAP SND acc) ++ MAP SND pfs
-Proof
-  Induct_on`pfs`>>rw[extract_clauses_def] >> simp[MAP_REVERSE]>>
-  every_case_tac>>fs[]>>
-  first_x_assum drule>>
-  rw[]
-QED
-
-Definition check_pbpstep_def:
-  (check_pbpstep (step:pbpstep) (fml:pbf) (id:num) =
-  case step of
+Definition check_lstep_def:
+  (check_lstep lstep (fml:pbf) (id:num) =
+  case lstep of
     Contradiction n =>
-      (case lookup n fml of
-        NONE => Fail
-      | SOME c =>
-        if check_contradiction c
-        then Unsat id
-        else Fail)
+    (case lookup n fml of
+      NONE => Fail
+    | SOME c =>
+      if check_contradiction c
+      then Unsat id
+      else Fail)
   | Check n c =>
     if lookup n fml = SOME c
     then Cont fml id
@@ -187,62 +113,18 @@ Definition check_pbpstep_def:
     | SOME c => Cont (insert id c fml) (id+1))
   | Con c pf =>
     let fml_not_c = insert id (not c) fml in
-    (case check_pbpsteps pf fml_not_c (id+1) of
+    (case check_lsteps pf fml_not_c (id+1) of
       Unsat id' => Cont (insert id' c fml) (id'+1)
-    | _ => Fail)
-  | Red c s pfs =>
-    (let fml_not_c = insert id (not c) fml in
-      let w = subst_fun s in
-      case extract_clauses w c fml pfs [] of
-        NONE => Fail
-      | SOME cpfs =>
-      (case check_redundancy cpfs fml_not_c (id+1) of
-        Cont fml' id' =>
-        let goals = MAP FST (toAList (map_opt (subst_opt w) fml)) in
-        let pids = MAP FST pfs in (* optimize and change later *)
-          if MEM (SOME (INR ())) pids ∧
-            EVERY (λid. MEM (SOME (INL id)) pids) goals then
-            Cont (insert id' c fml) (id'+1)
-          else Fail
-      | _ => Fail) )) ∧
-  (check_pbpsteps [] fml id = Cont fml id) ∧
-  (check_pbpsteps (step::steps) fml id =
-    case check_pbpstep step fml id of
-      Cont fml' id' => check_pbpsteps steps fml' id'
-    | res => res) ∧
-  (check_redundancy [] fml id = Cont fml id) ∧
-  (check_redundancy ((copt,pf)::pfs) fml id =
-    case copt of
-      NONE => (* no clause given *)
-      (if ~EVERY is_pol_con pf then Fail else
-      case check_pbpsteps pf fml id of
-        Cont fml' id' => check_redundancy pfs fml' id'
-      | res => Fail)
-    | SOME c =>
-      let cfml = insert id (not c) fml in
-      case check_pbpsteps pf cfml (id+1) of
-        Unsat id' => check_redundancy pfs fml id'
-      | res => Fail)
+    | _ => Fail)) ∧
+  (check_lsteps [] fml id = Cont fml id) ∧
+  (check_lsteps (step::steps) fml id =
+    case check_lstep step fml id of
+      Cont fml' id' => check_lsteps steps fml' id'
+    | res => res)
 Termination
   WF_REL_TAC ‘measure (
-    sum_size (pbpstep_size o FST)
-    (sum_size (list_size pbpstep_size o FST)
-    (list_size (list_size pbpstep_size) o MAP SND o FST)))’
-  \\ fs [fetch "-" "pbpstep_size_eq"] \\ rw []
-  >- (EVAL_TAC>>rw[])
-  >- (EVAL_TAC>>rw[])
-  >- (EVAL_TAC>>rw[])
-  >- (EVAL_TAC>>rw[])
-  \\ drule extract_clauses_MAP_SND
-  \\ simp[] \\ rw[]
-  \\ qmatch_goalsub_abbrev_tac`ls1 < _ + (_ + (ls2 + _))`
-  \\ `ls1 <= ls2` by (
-    unabbrev_all_tac
-    \\ rpt (pop_assum kall_tac)
-    \\ Induct_on`pfs` \\ simp[FORALL_PROD]
-    \\ rw[] \\ EVAL_TAC
-    \\ fs[])
-  \\ simp[]
+    sum_size (lstep_size o FST)
+    (list_size lstep_size o FST) )’
 End
 
 Theorem check_cutting_correct:
@@ -309,6 +191,16 @@ Proof
     metis_tac[compact_weaken])
 QED
 
+Definition id_ok_def:
+  id_ok fml id = ∀n. id ≤ n ⇒ n ∉ domain fml
+End
+
+Theorem sat_implies_refl[simp]:
+  fml ⊨ fml
+Proof
+  rw[sat_implies_def]
+QED
+
 Theorem range_FOLDL_delete:
   ∀ls v.
   range (FOLDL (λa b. delete b a) v ls) ⊆ range v
@@ -320,47 +212,20 @@ Proof
   simp[range_delete]
 QED
 
+Theorem sat_implies_subset:
+  s ⊆ t ⇒
+  t ⊨ s
+Proof
+  rw[sat_implies_def,satisfies_def,SUBSET_DEF]>>
+  metis_tac[]
+QED
+
 Theorem satisfiable_subset:
   satisfiable t ∧ s ⊆ t ⇒
   satisfiable s
 Proof
   rw[satisfiable_def,SUBSET_DEF,satisfies_def]>>
   metis_tac[]
-QED
-
-Theorem implies_explode:
-  a ⊨ s ⇔ ∀c. c ∈ s ⇒ a ⊨ {c}
-Proof
-  fs [sat_implies_def,satisfies_def]
-  \\ metis_tac []
-QED
-
-Theorem unsat_iff_implies:
-  ¬satisfiable (not x INSERT fml) ⇔ fml ⊨ {x}
-Proof
-  fs [sat_implies_def,satisfiable_def,not_thm]
-  \\ metis_tac []
-QED
-
-Definition id_ok_def:
-  id_ok fml id = ∀n. id ≤ n ⇒ n ∉ domain fml
-End
-
-Theorem lookup_mk_BS:
-  lookup i (mk_BS t1 a t2) = lookup i (BS t1 a t2)
-Proof
-  Cases_on ‘t1’ \\ Cases_on ‘t2’ \\ fs [mk_BS_def,lookup_def]
-QED
-
-Theorem lookup_map_opt:
-  ∀n t f.
-    lookup n (map_opt f t) =
-    case lookup n t of
-    | NONE => NONE
-    | SOME x => f x
-Proof
-  recInduct lookup_ind \\ fs [map_opt_def,lookup_def] \\ rw []
-  \\ rpt (fs [lookup_def,lookup_mk_BN,lookup_mk_BS] \\ CASE_TAC)
 QED
 
 Theorem id_ok_insert_1:
@@ -370,16 +235,201 @@ Proof
   rw[id_ok_def]
 QED
 
-Theorem unsat_satisfies_insert:
-  n ∉ domain fml ∧
-  id ∉ domain fml ∧
-  ¬satisfiable (range (insert n (not c) fml)) ⇒
-  range fml ⊨  range (insert id c fml)
+Theorem check_lstep_correct:
+  (∀step fml id.
+     id_ok fml id ⇒
+     case check_lstep step fml id of
+     | Cont fml' id' =>
+         id ≤ id' ∧
+         id_ok fml' id' ∧
+         range fml ⊨ range fml'
+     | Unsat id' =>
+        id ≤ id' ∧
+         ¬ satisfiable (range fml)
+     | Fail => T) ∧
+  (∀steps fml id.
+     id_ok fml id ⇒
+     case check_lsteps steps fml id of
+     | Cont fml' id' =>
+         id ≤ id' ∧
+         id_ok fml' id' ∧
+         range fml ⊨ range fml'
+     | Unsat id' =>
+        id ≤ id' ∧
+         ¬ satisfiable (range fml)
+     | Fail => T)
 Proof
-  fs[Once implies_explode,range_insert] \\ rw[]
-  \\ gs[range_insert,unsat_iff_implies]
-  \\ fs[sat_implies_def,satisfies_def]
+  ho_match_mp_tac check_lstep_ind \\ reverse (rpt strip_tac)
+  >- (
+    simp[Once check_lstep_def]>>
+    every_case_tac>>gs[]>>
+    metis_tac[sat_implies_def,satisfiable_def])
+  >-
+    simp[Once check_lstep_def]
+  \\ Cases_on ‘∃n. step = Contradiction n’
+  THEN1 (
+    rw[check_lstep_def] \\ every_case_tac \\ fs [] >>
+    rw[satisfiable_def,range_def,satisfies_def]>>
+    drule check_contradiction_unsat>>
+    metis_tac[])
+  \\ Cases_on ‘∃n c. step = Check n c’
+  THEN1
+   (rw[check_lstep_def] \\ every_case_tac \\ fs [] \\ metis_tac[sat_implies_refl])
+  \\ Cases_on ‘∃n. step = Delete n’
+  THEN1 (
+    rw[check_lstep_def] \\ every_case_tac \\ rw []
+    THEN1
+     (pop_assum mp_tac
+      \\ qid_spec_tac ‘fml’ \\ Induct_on ‘l’ \\ fs []
+      \\ rw [] \\ first_x_assum irule \\ fs [id_ok_def,domain_delete]) >>
+    match_mp_tac sat_implies_subset>>
+    fs[range_FOLDL_delete])
+  \\ Cases_on ‘step = NoOp’ >- simp[check_lstep_def]
+  \\ Cases_on ‘∃c. step = Cutting c’
+  THEN1 (
+    rw[check_lstep_def] \\ every_case_tac \\ rw []
+    THEN1 fs [id_ok_def] >>
+    drule check_cutting_correct>>
+    fs[satisfiable_def,satisfies_def]>>
+    ‘id ∉ domain fml’ by fs [id_ok_def]  >>
+    simp[sat_implies_def,satisfies_def]>>
+    fs [range_insert]>>
+    metis_tac[])
+  (* Proof by contradiction *)
+  \\ Cases_on ‘∃c steps. step = Con c steps’
+  THEN1 (
+    fs[check_lstep_def]
+    \\ every_case_tac \\ gs[id_ok_insert_1]
+    \\ `id_ok fml n` by fs[id_ok_def]
+    \\ fs[sat_implies_def,satisfies_def]
+    \\ `n ∉ domain fml’ by
+      fs [id_ok_def]
+    \\ simp[id_ok_insert_1, range_insert]
+    \\ fs[satisfiable_def,range_insert,id_ok_def,not_thm]
+    \\ metis_tac[satisfies_def])
+  THEN1 (
+    rw[Once check_lstep_def]
+    \\ every_case_tac \\ gvs [])
 QED
+
+Theorem check_lstep_compact:
+  (∀step fml id fml' id'.
+     (∀c. c ∈ range fml ⇒ compact c) ∧ lstep_ok step ∧
+     check_lstep step fml id = Cont fml' id' ⇒
+     (∀c. c ∈ range fml' ⇒ compact c)) ∧
+  (∀steps fml id fml' id'.
+     (∀c. c ∈ range fml ⇒ compact c) ∧ EVERY lstep_ok steps ∧
+     check_lsteps steps fml id = Cont fml' id' ⇒
+     (∀c. c ∈ range fml' ⇒ compact c))
+Proof
+  ho_match_mp_tac check_lstep_ind \\ reverse (rw [])
+  >- (
+    qpat_x_assum`_ = Cont _ _` mp_tac>>
+    simp[Once check_lstep_def]>>
+    every_case_tac>>fs[])
+  >- fs[Once check_lstep_def]>>
+  Cases_on`step`>>fs[check_lstep_def]>>
+  every_case_tac>>rw[]
+  >- metis_tac[range_FOLDL_delete,SUBSET_DEF]
+  >- (drule range_insert_2>>rw[]>>
+      metis_tac[check_cutting_compact])
+  \\ imp_res_tac range_insert_2 \\ gvs []
+QED
+
+Type subst = ``:(bool + num lit) num_map``;
+
+(* Steps that preserve satisfiability
+  TODO: add dominance here, which may necessitate some
+  changes to the representations *)
+Datatype:
+  sstep =
+  | Lstep lstep (* Id representing a contradiction *)
+  | Red npbc subst
+    (( (num + unit) option,lstep list) alist)
+    (* Ordered list of proofs for subgoals
+      NONE -> global subproof steps
+      SOME () -> the (currently) unique specific subgoal for Red
+      SOME n -> the subgoal for constraint id n
+    *)
+End
+
+(* Apply a substitution where needed *)
+Definition extract_clauses_def:
+  (extract_clauses f def fml [] acc = SOME (REVERSE acc)) ∧
+  (extract_clauses f def fml (cpf::pfs) acc =
+    case cpf of
+      (NONE,pf) => extract_clauses f def fml pfs ((NONE,pf)::acc)
+    | (SOME (INL n),pf) =>
+      (case lookup n fml of
+        NONE => NONE
+      | SOME c => extract_clauses f def fml pfs ((SOME (subst f c),pf)::acc))
+    | (SOME (INR u),pf) =>
+      extract_clauses f def fml pfs ((SOME (subst f def),pf)::acc))
+End
+
+Theorem extract_clauses_MAP_SND:
+  ∀f def fml pfs acc res.
+  extract_clauses f def fml pfs acc = SOME res ⇒
+  MAP SND res =  REVERSE (MAP SND acc) ++ MAP SND pfs
+Proof
+  Induct_on`pfs`>>rw[extract_clauses_def] >> simp[MAP_REVERSE]>>
+  every_case_tac>>fs[]>>
+  first_x_assum drule>>
+  rw[]
+QED
+
+(* TODO: could use Cont to return fml if needed...
+  But I think we just throw away the fml even for dominance *)
+Definition check_red_def:
+  (check_red [] fml id = SOME id) ∧
+  (check_red ((copt,pf)::pfs) fml id =
+    case copt of
+      NONE => (* no clause given *)
+      (case check_lsteps pf fml id of
+        Cont fml' id' => check_red pfs fml' id'
+      | res => NONE)
+    | SOME c =>
+      (let cfml = insert id (not c) fml in
+      case check_lsteps pf cfml (id+1) of
+        Unsat id' => check_red pfs fml id'
+      | res => NONE))
+End
+
+Definition subst_fun_def:
+  subst_fun (s:subst) n = lookup n s
+End
+
+Definition map_opt_def:
+  map_opt f LN = LN ∧
+  map_opt f (LS x) = (case f x of NONE => LN | SOME a => LS a) ∧
+  map_opt f (BN t1 t2) = mk_BN (map_opt f t1) (map_opt f t2) ∧
+  map_opt f (BS t1 x t2) =
+    case f x of
+    | NONE => mk_BN (map_opt f t1) (map_opt f t2)
+    | SOME a => mk_BS (map_opt f t1) a (map_opt f t2)
+End
+
+Definition check_sstep_def:
+  (check_sstep sstep (fml:pbf) (id:num) =
+  case sstep of
+    Lstep lstep =>
+    check_lstep lstep fml id
+  | Red c s pfs =>
+    (let fml_not_c = insert id (not c) fml in
+      let w = subst_fun s in
+      case extract_clauses w c fml pfs [] of
+        NONE => Fail
+      | SOME cpfs =>
+      (case check_red cpfs fml_not_c (id+1) of
+        SOME id' =>
+        let goals = MAP FST (toAList (map_opt (subst_opt w) fml)) in
+        let pids = MAP FST pfs in (* optimize and change later *)
+          if MEM (SOME (INR ())) pids ∧
+            EVERY (λid. MEM (SOME (INL id)) pids) goals then
+            Cont (insert id' c fml) (id'+1)
+          else Fail
+      | _ => Fail) ))
+End
 
 Theorem sat_implies_transitive:
   fml ⊨ fml' ∧ fml' ⊨ fml'' ⇒
@@ -388,10 +438,58 @@ Proof
   rw[sat_implies_def]
 QED
 
-Theorem sat_implies_refl:
-  fml ⊨ fml
+Theorem unsat_iff_implies:
+  ¬satisfiable (not x INSERT fml) ⇔ fml ⊨ {x}
 Proof
-  rw[sat_implies_def]
+  fs [sat_implies_def,satisfiable_def,not_thm]
+  \\ metis_tac []
+QED
+
+Theorem check_red_correct:
+  ∀pfs fml id.
+    id_ok fml id ⇒
+    case check_red pfs fml id of
+      SOME id' =>
+       id ≤ id' ∧
+       EVERY (λ(copt,pf).
+         case copt of
+           NONE => T
+         | SOME c => range fml ⊨ {c}
+       ) pfs
+    | NONE => T
+Proof
+  Induct>-rw[check_red_def]>>
+  Cases>>rw[check_red_def]>>
+  Cases_on`q`>>fs[]
+  >- (
+    every_case_tac>>fs[]>>
+    drule (CONJUNCT2 check_lstep_correct)>>
+    disch_then (qspec_then`r` assume_tac)>>
+    gs[]>>
+    first_x_assum drule>>simp[]>>
+    rw[]>>
+    pop_assum mp_tac>>
+    match_mp_tac MONO_EVERY>>
+    Cases>>simp[]>>every_case_tac>>
+    metis_tac[sat_implies_transitive])>>
+  every_case_tac>>fs[]>>
+  `id_ok (insert id (not x) fml) (id + 1)` by
+    fs[id_ok_def]>>
+  drule (CONJUNCT2 check_lstep_correct)>>
+  disch_then (qspec_then`r` assume_tac)>>
+  gs[]>>
+  `id_ok fml n` by
+    fs[id_ok_def]>>
+  first_x_assum drule>>
+  simp[]>>
+  gs[range_insert,id_ok_def,unsat_iff_implies]
+QED
+
+Theorem implies_explode:
+  a ⊨ s ⇔ ∀c. c ∈ s ⇒ a ⊨ {c}
+Proof
+  fs [sat_implies_def,satisfies_def]
+  \\ metis_tac []
 QED
 
 Theorem extract_clauses_MEM_acc:
@@ -436,200 +534,116 @@ Proof
   metis_tac[]
 QED
 
-Theorem check_pbpstep_correct:
-  (∀step fml id.
-     id_ok fml id ⇒
-     case check_pbpstep step fml id of
-     | Cont fml' id' =>
-         id ≤ id' ∧
-         id_ok fml' id' ∧
-         (satisfiable (range fml) ⇒ satisfiable (range fml')) ∧
-         (is_pol_con step ⇒ range fml ⊨ range fml')
-     | Unsat id' =>
-        id ≤ id' ∧
-         ¬ satisfiable (range fml)
-     | Fail => T) ∧
-  (∀steps fml id.
-     id_ok fml id ⇒
-     case check_pbpsteps steps fml id of
-     | Cont fml' id' =>
-        id ≤ id' ∧
-         id_ok fml' id' ∧
-         (satisfiable (range fml) ⇒ satisfiable (range fml')) ∧
-         (EVERY is_pol_con steps ⇒ range fml ⊨ range fml')
-     | Unsat id' =>
-        id ≤ id' ∧
-         ¬ satisfiable (range fml)
-     | Fail => T) ∧
-  (∀pfs fml id.
-     id_ok fml id ⇒
-     case check_redundancy pfs fml id of
-     | Cont fml' id' =>
-        id ≤ id' ∧
-        id_ok fml' id' ∧
-        (satisfiable (range fml) ⇒ satisfiable (range fml')) ∧
-        EVERY (λ(copt,pf).
-          case copt of
-            NONE => T
-          | SOME c => range fml ⊨ {c}
-        ) pfs
-     | _ => T)
+Theorem lookup_mk_BS:
+  lookup i (mk_BS t1 a t2) = lookup i (BS t1 a t2)
 Proof
-  ho_match_mp_tac check_pbpstep_ind \\ reverse (rpt strip_tac)
-  >- (
-    simp[Once check_pbpstep_def]>>
-    Cases_on`copt`>>fs[]
-    >- (
-      IF_CASES_TAC >- fs[]>>
-      qmatch_goalsub_abbrev_tac`check_pbpsteps stepss _ _`>>
-      Cases_on`check_pbpsteps stepss fml id` >> fs[]>>
-      gs[o_DEF,ETA_AX]>>rw[]>>
-      TOP_CASE_TAC>>fs[]>>
-      fs[EVERY_MEM]>>
-      rw[]>>first_x_assum drule>>
-      pairarg_tac>>simp[]>>
-      every_case_tac>>fs[]>>
-      metis_tac[sat_implies_transitive])>>
-    every_case_tac>>fs[]>>
-    gs[id_ok_insert_1]>>
-    qpat_x_assum`_ ⇒ _` mp_tac >>
-    impl_tac >- fs[id_ok_def]>>
-    rw[]>>
-    `id ∉ domain fml` by fs[id_ok_def]>>
-    fs[range_insert,id_ok_def]>>
-    metis_tac[unsat_iff_implies])
-  >- simp[check_pbpstep_def]
-  >- (
-    rw[Once check_pbpstep_def]
-    \\ every_case_tac \\ gvs []
-    \\ metis_tac[sat_implies_transitive])
-  >- (rw[Once check_pbpstep_def] >> metis_tac[sat_implies_refl])
-  \\ Cases_on ‘∃n. step = Contradiction n’
-  THEN1 (
-    rw[check_pbpstep_def] \\ every_case_tac \\ fs [] >>
-    rw[satisfiable_def,range_def,satisfies_def]>>
-    drule check_contradiction_unsat>>
-    metis_tac[])
-  \\ Cases_on ‘∃n c. step = Check n c’
-  THEN1
-   (rw[check_pbpstep_def] \\ every_case_tac \\ fs [] \\ metis_tac[sat_implies_refl])
-  \\ Cases_on ‘∃n. step = Delete n’
-  THEN1 (
-    rw[check_pbpstep_def] \\ every_case_tac \\ rw []
-    THEN1
-     (pop_assum mp_tac
-      \\ qid_spec_tac ‘fml’ \\ Induct_on ‘l’ \\ fs []
-      \\ rw [] \\ first_x_assum irule \\ fs [id_ok_def,domain_delete]) >>
-    drule satisfiable_subset>>
-    disch_then match_mp_tac>>
-    fs[range_FOLDL_delete])
-  \\ Cases_on ‘step = NoOp’ >- simp[check_pbpstep_def]
-  \\ Cases_on ‘∃c. step = Cutting c’
-  THEN1 (
-    rw[check_pbpstep_def] \\ every_case_tac \\ rw []
-    THEN1 fs [id_ok_def] >>
-    drule check_cutting_correct>>
-    fs[satisfiable_def,satisfies_def]>>
-    ‘id ∉ domain fml’ by fs [id_ok_def]  >>
-    fs [range_insert]
-    >- metis_tac []>>
-    simp[sat_implies_def,satisfies_def])
-  (* Proof by contradiction *)
-  \\ Cases_on ‘∃c steps. step = Con c steps’
-  THEN1 (
-    fs[check_pbpstep_def]
-    \\ every_case_tac \\ gs[id_ok_insert_1]
-    \\ `id_ok fml n` by fs[id_ok_def]
-    \\ simp[id_ok_insert_1]
-    \\ conj_asm2_tac
-    >- (
-      fs[satisfiable_def,sat_implies_def]>>
-      metis_tac[])
-    \\ match_mp_tac (GEN_ALL unsat_satisfies_insert)
-    \\ first_x_assum (irule_at Any)
-    \\ fs[id_ok_def])
-  (* Red steps *)
-  \\ cheat
-  (* TODO: something broken below
-  \\ ‘∃c s pfs. step = Red c s pfs’ by (Cases_on ‘step’ \\ fs [])
-  \\ gvs []
-  \\ simp[check_pbpstep_def]
-  \\ every_case_tac
-  \\ gs[id_ok_insert_1]
-  \\ CONJ_TAC >- gvs[id_ok_def]>>
-  qsuff_tac ‘c redundant_wrt (range fml)’
-  >- (
-    fs [redundant_wrt_def] \\ rw []
-    \\ irule satisfiable_subset
-    \\ pop_assum $ irule_at Any
-    \\ rw [SUBSET_DEF] \\ imp_res_tac range_insert_2 \\ fs [])
-  \\ rw[substitution_redundancy]
-  \\ qexists_tac ‘subst_fun s’ \\ fs []
-  \\ fs[EVERY_MEM,MEM_MAP,EXISTS_PROD]
-  \\ `id ∉ domain fml` by fs[id_ok_def]
-  \\ fs[range_insert]
-  \\ simp [Once implies_explode] \\ reverse (rw [])
-  THEN1 (
-    drule extract_clauses_MEM_INR
-    \\ strip_tac
-    \\ first_x_assum drule \\ strip_tac
-    \\ first_x_assum drule
-    \\ simp[]
-    \\ fs[lookup_insert]
-    \\ simp[Once INSERT_SING_UNION,UNION_COMM])
-  \\ gvs [GSYM unsat_iff_implies]
-  \\ pop_assum mp_tac
-  \\ simp [Once range_def] \\ rw []
-  \\ rename [‘lookup a fml = SOME xx’]
-  \\ fs [MEM_toAList,lookup_map_opt,CaseEq"option",PULL_EXISTS]
-  \\ last_x_assum drule
-  \\ Cases_on ‘subst_opt (subst_fun s) xx’ \\ fs []
-  THEN1
-   (imp_res_tac subst_opt_NONE
-    \\ CCONTR_TAC \\ gvs [satisfiable_def,not_thm]
-    \\ fs [satisfies_def,range_def,PULL_EXISTS]
-    \\ metis_tac[])
-  \\ strip_tac
-  \\  drule extract_clauses_MEM_INR
-  \\ strip_tac
-  \\ first_x_assum drule
-  \\ strip_tac
-  \\ first_x_assum drule
-  \\ fs[]
-  \\ metis_tac[INSERT_SING_UNION,UNION_COMM] *)
+  Cases_on ‘t1’ \\ Cases_on ‘t2’ \\ fs [mk_BS_def,lookup_def]
 QED
 
-Theorem check_pbpstep_compact:
-  (∀step fml id fml' id'.
-     (∀c. c ∈ range fml ⇒ compact c) ∧ pbpstep_ok step ∧
-     check_pbpstep step fml id = Cont fml' id' ⇒
-     (∀c. c ∈ range fml' ⇒ compact c)) ∧
-  (∀steps fml id fml' id'.
-     (∀c. c ∈ range fml ⇒ compact c) ∧ EVERY pbpstep_ok steps ∧
-     check_pbpsteps steps fml id = Cont fml' id' ⇒
-     (∀c. c ∈ range fml' ⇒ compact c)) ∧
-  (∀pfs fml id fml' id'.
-     (∀c. c ∈ range fml ⇒ compact c) ∧
-     EVERY (EVERY pbpstep_ok) (MAP SND pfs) ∧
-     check_redundancy pfs fml id = Cont fml' id' ⇒
-     (∀c. c ∈ range fml' ⇒ compact c))
+Theorem lookup_map_opt:
+  ∀n t f.
+    lookup n (map_opt f t) =
+    case lookup n t of
+    | NONE => NONE
+    | SOME x => f x
 Proof
-  ho_match_mp_tac check_pbpstep_ind \\ reverse (rw [])
+  recInduct lookup_ind \\ fs [map_opt_def,lookup_def] \\ rw []
+  \\ rpt (fs [lookup_def,lookup_mk_BN,lookup_mk_BS] \\ CASE_TAC)
+QED
+
+Theorem check_sstep_correct:
+  ∀step fml id.
+  id_ok fml id ⇒
+  case check_sstep step fml id of
+  | Cont fml' id' =>
+      id ≤ id' ∧
+      id_ok fml' id' ∧
+      (satisfiable (range fml) ⇒ satisfiable (range fml'))
+  | Unsat id' =>
+     id ≤ id' ∧
+      ¬ satisfiable (range fml)
+  | Fail => T
+Proof
+  Cases>>rw[check_sstep_def]
   >- (
-    gs[Once check_pbpstep_def,AllCaseEqs()]>>
-    gs[o_DEF,ETA_AX])
-  >- fs[Once check_pbpstep_def]
-  THEN1
-   (ntac 2 (pop_assum mp_tac)
-    \\ simp [Once check_pbpstep_def,AllCaseEqs()]
-    \\ rw [] \\ fs [])
-  THEN1 (fs [Once check_pbpstep_def,AllCaseEqs()]) >>
-  Cases_on`step`>>fs[check_pbpstep_def]>>
-  every_case_tac>>rw[]
-  >- metis_tac[range_FOLDL_delete,SUBSET_DEF]
-  >- (drule range_insert_2>>rw[]>>
-      metis_tac[check_cutting_compact])
-  \\ imp_res_tac range_insert_2 \\ gvs []
+    drule (CONJUNCT1 check_lstep_correct)>>
+    disch_then(qspec_then `l` assume_tac)>>
+    every_case_tac>>fs[]>>
+    fs[satisfiable_def,sat_implies_def]>>
+    metis_tac[])
+  >- ( (* Red *)
+    every_case_tac>>
+    gs[id_ok_insert_1]>>
+    `id_ok (insert id (not p) fml) (id + 1)` by
+      fs[id_ok_def]>>
+    drule check_red_correct>>
+    disch_then(qspec_then`x` assume_tac)>>gs[]>>
+    CONJ_TAC>-
+      gvs[id_ok_def]>>
+    rename1`insert id' c fml`>>
+    qsuff_tac ‘c redundant_wrt (range fml)’
+    >- (
+      fs [redundant_wrt_def] \\ rw []
+      \\ irule satisfiable_subset
+      \\ pop_assum $ irule_at Any
+      \\ rw [SUBSET_DEF] \\ imp_res_tac range_insert_2 \\ fs [])
+    \\ rw[substitution_redundancy]
+    \\ qexists_tac ‘subst_fun s’ \\ fs []
+    \\ fs[EVERY_MEM,MEM_MAP,EXISTS_PROD]
+    \\ `id ∉ domain fml` by fs[id_ok_def]
+    \\ fs[range_insert]
+    \\ simp [Once implies_explode] \\ reverse (rw [])
+    THEN1 (
+      drule extract_clauses_MEM_INR
+      \\ strip_tac
+      \\ first_x_assum drule \\ strip_tac
+      \\ first_x_assum drule
+      \\ simp[]
+      \\ fs[lookup_insert]
+      \\ simp[Once INSERT_SING_UNION,UNION_COMM])
+    \\ gvs [GSYM unsat_iff_implies]
+    \\ pop_assum mp_tac
+    \\ simp [Once range_def] \\ rw []
+    \\ rename [‘lookup a fml = SOME xx’]
+    \\ fs [MEM_toAList,lookup_map_opt,CaseEq"option",PULL_EXISTS]
+    \\ last_x_assum drule
+    \\ Cases_on ‘subst_opt (subst_fun s) xx’ \\ fs []
+    THEN1
+     (imp_res_tac subst_opt_NONE
+      \\ CCONTR_TAC \\ gvs [satisfiable_def,not_thm]
+      \\ fs [satisfies_def,range_def,PULL_EXISTS]
+      \\ metis_tac[])
+    \\ Cases_on`x'` \\ fs[]
+    \\ strip_tac
+    \\ drule extract_clauses_MEM_INL
+    \\ disch_then drule
+    \\ strip_tac
+    \\ first_x_assum drule
+    \\ gvs[]
+    \\ metis_tac[INSERT_SING_UNION,UNION_COMM])
+QED
+
+Definition sstep_ok_def[simp]:
+  (sstep_ok (Lstep l) ⇔ lstep_ok l) ∧
+  (sstep_ok (Red n _ pfs) ⇔
+    compact n)
+  (* TODO: should this be added?
+  it checks that the subproofs are compact...
+  ∧ EVERY (EVERY lstep_ok) (MAP SND pfs)) *)
+End
+
+Theorem check_sstep_compact:
+  ∀sstep fml id fml' id'.
+  (∀c. c ∈ range fml ⇒ compact c) ∧ sstep_ok sstep ∧
+  check_sstep sstep fml id = Cont fml' id' ⇒
+  (∀c. c ∈ range fml' ⇒ compact c)
+Proof
+  Cases>>rw[]>>fs[check_sstep_def]
+  >-
+    metis_tac[check_lstep_compact] >>
+  every_case_tac>>gvs[]>>
+  drule range_insert_2>>rw[]>>
+  metis_tac[]
 QED
 
 val _ = export_theory ();
